More refactoring.
MATTHIEU: I moved some stuff from L3 to Ast.Common, and made it
parametric on the language (L0 - L3).  In order to make L3_to_L4.v and
L3_to_L4_correct.v check I added a few long pathnames and parameter
arguments.

L5 MAINTAINER: I'm not sure why L5 refers to things in L3, but in
order to make some examples at the end of cpseval.v check, I changed
some type cast annotations.

certicoq/theories/L2_typeStripped/compile.v
@@ -99,7 +99,6 @@ Function stripEC (ec:L1_5EC) : envClass :=
   match ec with
     | AstCommon.ecTrm t => AstCommon.ecTrm (strip t)
     | AstCommon.ecTyp _ n itp => AstCommon.ecTyp Term n itp
-    | AstCommon.ecAx _ => AstCommon.ecAx Term
   end.
 
 Definition  stripEnv : L1_5Env -> environ :=
