certicoq/theories/L5_CPS/cpseval.v
@@ -499,9 +499,9 @@ Definition typedef := ((fun (A:Type) (a:A) => a) Nat 1%nat).
 Quote Definition q_typedef := Eval compute in typedef.
 Quote Recursively Definition p_typedef := typedef.
 Eval compute in (compile.program_Program p_typedef :
-                   exception compile.Program).
+                   exception (Program compile.Term)).
 
-Definition L1_typedef : exception compile.Program :=
+Definition L1_typedef  :=
   Eval compute in compile.program_Program p_typedef.
 
 Definition P_typedef := Eval compute in program_exp p_typedef.
